theories/TM/Single/DecodeTapes.v
@@ -30,8 +30,8 @@ Module CheckEncodeTapes.
                  /\ exists t1 b1, ContainsEncoding.Rel (Encode_tape sig) Retr_f [|tape_move_right t|] (b1,t1)
                             /\ if b1 then R_syntactic n (tape_move_right t1[@Fin0]) b t'
                               else t1[@Fin0]=t' /\ b = false)
-                \/ (Option.bind Retr_g (current t) <> Some sigList_cons /\ b = false)
-        end.
+                \/ (Option.bind Retr_g (current t) <> Some sigList_cons /\ b = false /\ t=t')
+        end .
     
     Fixpoint M n : pTM tau bool 1 :=
       match n with
@@ -41,7 +41,7 @@ Module CheckEncodeTapes.
                  (Return Nop false)
       end.
 
-    Lemma Realises n: M n ⊨ (fun t '(b,t') => R_syntactic n t[@Fin0] b t'[@Fin0]).
+    Lemma Realises_intern n: M n ⊨ (fun t '(b,t') => R_syntactic n t[@Fin0] b t'[@Fin0]).
     Proof.
       induction n.
       -cbn. eapply Realise_monotone. now TM_Correct.
@@ -51,44 +51,88 @@ Module CheckEncodeTapes.
        destruct (Option.bind Retr_g (current t'[@Fin0])) as [ [] | ]. all:subst b;constructor. all:easy.
       -cbn. eapply Realise_monotone.
        { TM_Correct. now apply CheckEncodesTape.Realises. eassumption. }
-       hnf;cbn. intros t (b,t') [H|H].
-       2:{ right.  destruct H as (?&(?&Hb&->&->)&->&_&<-). split. 2:easy. intros H. rewrite H in Hb. easy. }
-       left. destruct H as (?&(?&Hb&->&->)&_&tmp&->&H). clear tmp.
+       hnf;cbn. intros t (b,t') [H|H]. 
+       2:{ destruct H as (?&(?&Hb&->&->)&->&_&<-). right. split. 2:easy. intros H. rewrite H in Hb. easy. }
+       destruct H as (?&(?&Hb&->&->)&_&tmp&Htmp&H). unfold tapes in tmp. destruct_vector. cbn in Htmp. subst h.
        decide (Option.bind Retr_g (current t[@Fin0]) = Some sigList_cons) as [Ht|Ht].
-       2:now destruct Option.bind as [[]| ]. split. easy.
+       2:now destruct Option.bind as [[]| ]. left. split. easy.
        destruct H as [(t1&Ht1&?&?&->&Rsynt)|(?&Ht'&->&_&<-)].
-       2:{ eexists _,false. split. 2:easy. cbn. now apply CheckEncodesTape.f_spec in Ht'. }
-       eexists _,true. split. 1:{ apply CheckEncodesTape.f_spec in Ht1. exact Ht1. }
-       easy.
+       2:{ eexists _,false. split. 2:easy. easy. }
+       eexists _,true. split. eassumption. easy.
     Qed.
 
+    From Undecidability Require Import LTactics.
+    
+    Definition Ter n : tRel tau 1:=
+      fun t k => n * ((| right t[@Fin0] |) * 4 + 9 + 7) + 1 <= k.
+    
+    (*MOVE*)
+    Lemma iter_transitive X Y R (g:X -> Y) f s n: PreOrder R ->  (forall x, R (g (f x)) (g x)) -> R (g (nat_rect _ s (fun _ => f) n)) (g s).
+    Proof.
+      intros Ht HR. induction n;cbn. easy. now etransitivity.
+    Qed.
+
+    (*MOVE*)
+    Lemma length_right_tape_move_right sig' (t : tape sig'): | right (tape_move_right t) | <= | right t |.
+    Proof.
+      destruct t eqn:Ht;cbn. 1-3:nia. now destruct l0;cbn.
+    Qed.
+      
+    Lemma Terminates n: projT1 (M n) ↓ Ter n. 
+    Proof.
+      unfold Ter.
+      induction n.
+      -cbn. eapply TerminatesIn_monotone. now TM_Correct.
+       intros ? ? ?. nia.
+      -assert (Ht:= length_right_tape_move_right).
+       cbn - [plus mult]. eapply TerminatesIn_monotone.
+       {TM_Correct. now apply CheckEncodesTape.Realises. now apply CheckEncodesTape.Terminates. eassumption. }
+       intros ? ? HT. set (n0:= | tape_local x[@Fin0] |) in *. cbn. infTer 5.
+        2:{ intros t ? (?&->&->&<-). destruct _.
+            infTer 5.  unfold CheckEncodesTape.Ter. intros ? _ Htout. rewrite !Htout. infTer 4.
+            intros ? ? ?. destruct b.
+            -infTer 5. intros ? ? ->.
+             rewrite !Ht. cbn in *. fold n0.  destruct H as [_ (k&H)].
+             rewrite H. rewrite iter_transitive with (g:=fun x => | right x |) (R:=le). 2:easy. 2:apply Ht.
+             rewrite Htout,Ht. fold n0. reflexivity.
+            -nia.
+            -nia.
+        }
+        ring_simplify. rewrite !Ht. fold n0. rewrite <- HT. ring_simplify. nia.
+    Qed.
+    
     Lemma R_syntactic__spec n t b t':
       R_syntactic n t b t'
       -> Rel n [|t|] (b,[|t'|]).
     Proof.
       unfold Rel,ContainsEncoding.Rel. unfold encode,Encode_tapes,encode_tapes. cbn.
       induction n in t |-*;cbn [R_syntactic].
-      {unfold Rel, ContainsEncoding.Rel. intros [[Hb] <-]. destruct Hb.
+      {unfold Rel, ContainsEncoding.Rel. intros [[Hb] <-]. split. 2:now eexists 0. destruct Hb.
        -destruct t;inv e. apply retract_g_inv in H0 as ->.
         eexists [||],_,_. cbn. split. now eexists _,[]. now eexists [],_.
        -intros ? v ?. rewrite (destruct_vector_nil v);cbn.
         eexists _,_. split. easy. intros ->. cbn in n. now retract_adjoint.
       }
-      intros [(Ht&t1&b1&HR&Hb1) | (Ht&->)].
-      2:{ clear IHn. cbn in *. intros ? v ?. destruct (destruct_vector_cons v) as (t0&b'&->). cbn.
+      intros [(Ht&t1&b1&HR&Hb1) | (Ht&->&->)].
+      2:{ clear IHn. cbn in *. split. 2:now eexists 0. intros ? v ?. destruct (destruct_vector_cons v) as (t0&b'&->). cbn.
           do 3 eexists. reflexivity. intros ->. cbn in Ht. now retract_adjoint. }
-      cbn. destruct b1;hnf in HR. 
-      2:{ clear IHn. destruct Hb1 as [<- ->]. intros ? v ?. destruct (destruct_vector_cons v) as (t0&b'&->). cbn.
+      cbn. destruct HR as (HR&(k & Ht1)). destruct b1;hnf in HR.
+      2:{ clear IHn. destruct Hb1 as [<- ->]. split. 2:{ exists (S k). now rewrite Ht1,nat_rect_succ_r. }
+          intros ? v ?. destruct (destruct_vector_cons v) as (t0&b'&->). cbn.
           do 3 eexists. easy. intros ->. cbn in HR.
           edestruct HR with (x:=t0) as (?&?&Hhd&Henc).
           destruct (encode_tape t0) eqn:Ht0. all:inv Hhd. cbn in Henc.
           apply Henc. unfold retr_comp_f. cbn. autorewrite with list. rewrite map_map. reflexivity. }
       cbn in HR. revert Ht. destruct t as [ | | | t__L c t__R];intros [= ->%retract_g_inv].
-      destruct HR as (t0&t__L'&t__R'&(x__hd&x__tl&eq__hd&Ht)&(x__init&x__last&eq__last&Ht')). rewrite Ht' in Hb1. clear t1 Ht'.
+      destruct HR as (t0&t__L'&t__R'&(x__hd&x__tl&eq__hd&Ht)&(x__init&x__last&eq__last&Ht')). rewrite Ht' in Hb1,Ht1. clear t1 Ht'.
       destruct t__R; inv Ht. cbn in Hb1. specialize IHn with (1:=Hb1);cbn in IHn.
+      destruct IHn as [IHn Hres].
+      split. 2:{ destruct Hres as [k' ->]. cbn. eexists (S ((S _) + _)). rewrite nat_rect_succ_r. cbn - [nat_rect plus]. rewrite nat_rect_plus.
+                  cbn in Ht1. rewrite <- Ht1. rewrite nat_rect_succ_r. now cbn. } clear Hres.
       destruct b.
       -destruct IHn as (v&t__Lv&t__Rv&(x__hd'&x__tl'&eq__hd'&Ht)&(x__init'&x__last'&eq__last'&->)).
-       destruct t__R' as [ |? t__R'];inv Ht. eexists (t0:::v),_,_;split.
+       destruct t__R' as [ |? t__R'];inv Ht. cbn in Ht1.
+       eexists (t0:::v),_,_;split.
        +cbn. do 3 eexists. reflexivity. rewrite eq__hd, eq__hd'. unfold retr_comp_f. cbn;autorewrite with list;cbn. rewrite map_map. easy.
        +cbn. rewrite eq__last, eq__last'. unfold retr_comp_f. cbn;autorewrite with list;cbn.
         eexists (_::_++_::_),_. split. 1:{ repeat (cbn;autorewrite with list). easy. }
@@ -104,6 +148,13 @@ Module CheckEncodeTapes.
        edestruct IHn as (?&?&?&Hneq). apply Hneq. cbn. rewrite H. cbn.
        f_equal.
     Qed.
+
+    Lemma Realises n: M n ⊨ Rel n.
+    Proof.
+      eapply Realise_monotone. now apply Realises_intern. intros t [? t'] ?%R_syntactic__spec.
+      unfold tapes in *. destruct_vector. easy.
+    Qed.
+          
     
   End checkEncodeTapes.
 End CheckEncodeTapes.
